A working solution but without an appropriate proof goal

chapter08-application-correspondence/solutions/exercise01_solution.dfy
@@ -6,7 +6,7 @@
 include "../../chapter07-async-clients/solutions/exercise01_solution.dfy" //#magicinline
 
 // For reference, go see your or the instructors' solution to chapter06-refine/exercises/exercise01.dfy
-module AsyncShardedKVProtocol {
+module AsyncClientShardedKVProtocol {
   import opened Library
   import opened Types
 
@@ -120,5 +120,400 @@ module AsyncShardedKVProtocol {
   predicate Next(c: Constants, v: Variables, v': Variables)
   {
     exists step :: NextStep(c, v, v', step)
+  }
+}
+
+module RefinementProof {
+  import opened Library
+  import opened Types
+  import MapSpec
+  import opened AsyncClientShardedKVProtocol
+
+  predicate HostHasKey(c: Constants, v: Variables, hostidx:HostIdx, key:Key)
+    requires v.WF(c)
+  {
+    && c.ValidHost(hostidx)
+    && key in v.maps[hostidx]
+  }
+
+  // Pulling the choose out into its own function is sometimes necessary due
+  // to a (deliberate) stupidity in Dafny: it doesn't treat :| expressions
+  // as subsitution-equivalent, even though the are (as evidenced by pulling
+  // one into a function).
+  function KeyHolder(c: Constants, v: Variables, key:Key) : HostIdx
+    requires v.WF(c)
+    requires exists hostidx :: HostHasKey(c, v, hostidx, key)
+  {
+    var hostidx:HostIdx :| HostHasKey(c, v, hostidx, key);
+    hostidx
+  }
+
+
+  function AbstractionOneKey(c: Constants, v: Variables, key:Key) : Value
+    requires v.WF(c)
+  {
+//#exercise    DefaultValue() // Replace me
+//#start-elide
+    if exists idx :: HostHasKey(c, v, idx, key)
+    then
+      v.maps[KeyHolder(c, v, key)][key]
+    else DefaultValue()
+//#end-elide
+  }
+
+  // We construct the finite set of possible map keys here, all
+  // because we need to supply Dafny with simple evidence that our map domain
+  // is finite for the map comprehension in Abstraction().
+  // (An alternative would be to switch to imaps -- maps with potentially-infinite
+  // domains -- but that would require making the spec fancier. This was a compromise.)
+
+  // The sequence of map domains. Pulled out into its own function to
+  // make proof assertions easy to write.
+  function MapDomains(c: Constants, v: Variables) : seq<set<Key>>
+    requires v.WF(c)
+  {
+    seq(c.mapCount, i requires 0<=i<c.mapCount => v.maps[i].Keys)
+  }
+
+  function KnownKeys(c: Constants, v: Variables) : set<Key>
+    requires v.WF(c)
+  {
+    UnionSeqOfSets(MapDomains(c, v))
+  }
+
+  // Packaged as lemma. Proves trivially as ensures of KnownKeys,
+  // but creates a trigger storm.
+  lemma HostKeysSubsetOfKnownKeys(c: Constants, v: Variables, count: nat)
+    requires v.WF(c)
+    requires count <= c.mapCount
+    ensures forall idx | 0 <= idx < count :: v.maps[idx].Keys <= KnownKeys(c, v)
+  {
+    forall idx | 0 <= idx < count ensures v.maps[idx].Keys <= KnownKeys(c, v)
+    {
+      SetsAreSubsetsOfUnion(MapDomains(c, v));
+      assert v.maps[idx].Keys == MapDomains(c, v)[idx];  // trigger
+    }
+  }
+
+  function Abstraction(c: Constants, v: Variables) : MapSpec.Variables
+    requires v.WF(c)
+  {
+//#exercise    MapSpec.Variables(InitialMap()) // Replace me
+//#start-elide
+    MapSpec.Variables(
+      map key | key in KnownKeys(c, v) :: AbstractionOneKey(c, v, key),
+      v.requests,
+      v.replies)
+//#end-elide
+  }
+
+//#elide  // This does slow things down quite a bit.
+  // This definition is useful, but a bit trigger-happy, so we made it
+  // opaque. This means that its body is hidden from Dafny, unless you
+  // explicitly write "reveal_KeysHeldUniquely();", at which point the
+  // body of the predicate becomes available within the current context
+  predicate {:opaque} KeysHeldUniquely(c: Constants, v: Variables)
+    requires v.WF(c)
+  {
+    forall key, hostidx:HostIdx, otherhost:HostIdx
+        | && c.ValidHost(hostidx) && c.ValidHost(otherhost)
+          && key in v.maps[hostidx] && key in v.maps[otherhost]
+        :: hostidx == otherhost
+  }
+
+  predicate Inv(c: Constants, v: Variables)
+  {
+//#exercise    false // Replace me
+//#start-elide
+    && v.WF(c)
+    // Every key lives somewhere.
+    && KnownKeys(c, v) == Types.AllKeys()
+    // No key lives in two places.
+    && KeysHeldUniquely(c, v)
+//#end-elide
+  }
+
+//#start-elide
+  lemma InitAllKeysEmpty(c: Constants, v: Variables, count: nat)
+    requires Init(c, v)
+    requires 0 < count <= c.mapCount
+    ensures KnownKeys(c, v) == AllKeys()
+  {
+    EachUnionMemberBelongsToASet(MapDomains(c, v));
+    SetsAreSubsetsOfUnion(MapDomains(c, v));
+    forall key | key in AllKeys() ensures key in KnownKeys(c, v) {
+      assert key in MapDomains(c,v)[0]; // trigger
+    }
+  }
+
+//#end-elide
+  lemma RefinementInit(c: Constants, v: Variables)
+    requires c.WF()
+    requires Init(c, v)
+    ensures MapSpec.Init(Abstraction(c, v))
+    ensures Inv(c, v)
+  {
+//#start-elide
+    InitAllKeysEmpty(c, v, c.mapCount);
+    reveal_KeysHeldUniquely();
+//#end-elide
+  }
+
+  // Since we know that keys are held uniquely, if we've found a host that holds a key, 
+  // that can be the only solution to the 'choose' operation that defines KeyHolder.
+  lemma AnyHostWithKeyIsKeyHolder(c: Constants, v: Variables, hostidx:HostIdx, key:Key)
+    requires v.WF(c)
+    requires KeysHeldUniquely(c, v)
+    requires HostHasKey(c, v, hostidx, key)
+    ensures KeyHolder(c, v, key) == hostidx
+  {
+    reveal_KeysHeldUniquely();
+  }
+
+  // This is not a goal by itself, it's one of the cases you'll need to prove
+  // NextPreservesInvAndRefines. We've provided its signature to help you
+  // structure your overall proof.
+  lemma InsertPreservesInvAndRefines(c: Constants, v: Variables, v': Variables, insertHost: HostIdx, request:Input)
+    requires Inv(c, v)
+    requires Next(c, v, v')
+    requires c.ValidHost(insertHost)
+    requires Insert(c, v, v', insertHost, request)
+    ensures Inv(c, v')
+    ensures MapSpec.Next(Abstraction(c, v), Abstraction(c, v'))
+  {
+//#start-elide
+    var abstractMap := Abstraction(c, v).mapp;
+    var abstractMap' := Abstraction(c, v').mapp;
+    var insertedKey := request.key; // use some let-in assignments to recycle chapter06 proof...
+    var value := request.value;
+
+    assert insertedKey in AllKeys() by {
+      SetsAreSubsetsOfUnion(MapDomains(c, v));
+      assert MapDomains(c, v)[insertHost] == v.maps[insertHost].Keys; //trigger
+    }
+
+    assert KeysHeldUniquely(c, v') by { reveal_KeysHeldUniquely(); }
+
+    forall key
+      ensures key in abstractMap' <==> key in abstractMap || key == insertedKey // domain
+      ensures key in abstractMap' ==> (abstractMap'[key] == if key==insertedKey then value else abstractMap[key])  // value
+    {
+      if key == insertedKey {
+        SetsAreSubsetsOfUnion(MapDomains(c, v'));
+        assert MapDomains(c, v')[insertHost] <= KnownKeys(c, v'); // trigger
+        assert key in abstractMap'; // case goal
+      }
+      if key in abstractMap {
+        var idx := GetIndexForMember(MapDomains(c, v), key);
+        assert MapDomains(c, v')[idx] <= KnownKeys(c, v') by {
+          // The lemma below is a trigger-trap danger (causes timeouts), so I'm
+          // careful to only call it tucked way into this by clause.
+          SetsAreSubsetsOfUnion(MapDomains(c, v'));
+        }
+        assert key in abstractMap'; // case goal
+      }
+      if key in abstractMap' {
+        if key == insertedKey {
+          AnyHostWithKeyIsKeyHolder(c, v', insertHost, key);
+          assert abstractMap'[key] == value;  // case goal
+        } else {
+          var keyIdx := GetIndexForMember(MapDomains(c, v'), key);
+          AnyHostWithKeyIsKeyHolder(c, v', keyIdx, key);
+          AnyHostWithKeyIsKeyHolder(c, v, keyIdx, key);
+          assert key in abstractMap by {
+            SetsAreSubsetsOfUnion(MapDomains(c, v));
+            assert MapDomains(c, v)[keyIdx] <= KnownKeys(c, v);  // trigger
+          }
+          assert abstractMap'[key] == abstractMap[key]; // case goal
+        }
+      }
+    }
+
+    assert KnownKeys(c, v') == Types.AllKeys() by {
+      assert abstractMap'.Keys == KnownKeys(c, v'); // trigger
+    }
+    assert MapSpec.NextStep(Abstraction(c, v), Abstraction(c, v'), MapSpec.InsertOpStep(request)); // witness
+//#end-elide
+  }
+
+  lemma ExistsHostHasKey(c:Constants, v:Variables, key:Key)
+    requires Inv(c, v)
+    requires key in KnownKeys(c, v);
+    ensures exists hostidx :: HostHasKey(c, v, hostidx, key)
+  {
+    EachUnionMemberBelongsToASet(MapDomains(c, v));
+//    assert key in UnionSeqOfSets(MapDomains(c, v));
+//    assert exists idx :: 0<=idx<c.mapCount && key in MapDomains(c, v)[idx];
+    var idx :| 0<=idx<c.mapCount && key in MapDomains(c, v)[idx];
+    assert HostHasKey(c, v, idx, key);
+  }
+
+  // This proof's interaction with automation gets a little clumsier with the
+  // addition of new fields to AsyncClientShardedKVProtocol.Variables. In
+  // chapter06, if v'.maps==v.maps, then v'==v, so it knew
+  // KeysHeldUniquely(v')==KeysHeldUniquely(v') just by substitution, even
+  // thought it couldn't see inside that predicate because it's {:opaque}.  Now
+  // we can have equal maps, but v'!=v because we fiddled with the
+  // requests/replies fields (as in Query), and Dafny can't tell that the
+  // predicate is identical.
+  // The instructors' minimal-edit solution was to prove these lemmas and use
+  // them as needed.
+  // Another more elegant possibility would be to redefine KeysHeldUniquely and
+  // related functions to only accept the maps field as an argument, so that
+  // Dafny could continue reasoning about them using only substitution. That
+  // would entail plumbing through some new maps-specific WF conditions as well.
+  lemma EqualMapsEqualKeysHeldUniquely(c: Constants, v: Variables, v': Variables)
+    requires v.WF(c)
+    requires v'.WF(c)
+    requires v'.maps == v.maps
+    ensures KeysHeldUniquely(c, v') == KeysHeldUniquely(c, v)
+  {
+    reveal_KeysHeldUniquely();
+  }
+
+  lemma EqualMapsEqualMapp(c: Constants, v: Variables, v': Variables)
+    requires Inv(c, v)
+    requires Inv(c, v')
+    requires v'.maps == v.maps
+    ensures Abstraction(c, v').mapp == Abstraction(c, v).mapp
+  {
+    forall k | k in Abstraction(c, v').mapp ensures Abstraction(c, v').mapp[k] == Abstraction(c, v).mapp[k] {
+      ExistsHostHasKey(c, v', k);
+      ExistsHostHasKey(c, v, k);
+      assert KeyHolder(c, v', k) == KeyHolder(c, v, k) by { reveal_KeysHeldUniquely(); }
+    }
+  }
+
+  // This is not a goal by itself, it's one of the cases you'll need to prove
+  // NextPreservesInvAndRefines. We've provided its signature to help you
+  // structure your overall proof.
+  lemma QueryPreservesInvAndRefines(c: Constants, v: Variables, v': Variables, queryHost: HostIdx, request: Input, output: Value)
+    requires Inv(c, v)
+    requires Next(c, v, v')
+    requires c.ValidHost(queryHost)
+    requires Query(c, v, v', queryHost, request, output)
+    ensures Inv(c, v')
+    ensures MapSpec.Next(Abstraction(c, v), Abstraction(c, v'))
+  {
+//#start-elide
+    var key := request.key;
+    assert v.maps == v'.maps; // weirdly obvious trigger
+    assert Inv(c, v') by { reveal_KeysHeldUniquely(); }
+    assert key in KnownKeys(c, v) by { HostKeysSubsetOfKnownKeys(c, v, c.mapCount); }
+    assert output == Abstraction(c, v).mapp[key] by {
+      assert HostHasKey(c, v, queryHost, key);  // witness
+      reveal_KeysHeldUniquely();
+    }
+    EqualMapsEqualMapp(c, v, v');
+    assert MapSpec.NextStep(Abstraction(c, v), Abstraction(c, v'), MapSpec.QueryOpStep(request, output)); // witness
+//#end-elide
+  }
+
+  // This is not a goal by itself, it's one of the cases you'll need to prove
+  // NextPreservesInvAndRefines. We've provided its signature to help you
+  // structure your overall proof.
+  lemma TransferPreservesInvAndRefines(c: Constants, v: Variables, v': Variables, sendIdx: HostIdx, recvIdx: HostIdx, sentKey: Key, value: Value)
+    requires Inv(c, v)
+    requires Next(c, v, v')
+    requires c.ValidHost(sendIdx)
+    requires c.ValidHost(recvIdx)
+    requires Transfer(c, v, v', sendIdx, recvIdx, sentKey, value)
+    ensures Inv(c, v')
+    ensures MapSpec.Next(Abstraction(c, v), Abstraction(c, v'))
+  {
+//#start-elide
+    // domain preserved
+    forall key
+      ensures key in Abstraction(c, v).mapp <==> key in Abstraction(c, v').mapp
+    {
+      var idx;
+      if key in Abstraction(c, v).mapp {
+        SetsAreSubsetsOfUnion(MapDomains(c, v'));
+        if key==sentKey {
+          idx := recvIdx;
+        }
+        else {
+          idx := GetIndexForMember(MapDomains(c, v), key);
+        }
+        assert MapDomains(c, v')[idx] <= KnownKeys(c, v');  // trigger
+        assert key in Abstraction(c, v').mapp;  // case goal
+      }
+      if key in Abstraction(c, v').mapp {
+        SetsAreSubsetsOfUnion(MapDomains(c, v));
+        if key==sentKey {
+          idx := sendIdx;
+        }
+        else {
+          idx := GetIndexForMember(MapDomains(c, v'), key);
+        }
+        assert MapDomains(c, v)[idx] <= KnownKeys(c, v);  // trigger
+        assert key in Abstraction(c, v).mapp;  // case goal
+      }
+    }
+
+    assert KeysHeldUniquely(c, v') by { reveal_KeysHeldUniquely(); }
+
+    // values preserved
+    forall key | key in Abstraction(c, v).mapp
+      ensures Abstraction(c, v).mapp[key] == Abstraction(c, v').mapp[key]
+    {
+      // identify where to find key in the old & new worlds
+      var idx, idx';
+      if key == sentKey {
+        idx := sendIdx;
+        idx' := recvIdx;
+      } else {
+        idx := GetIndexForMember(MapDomains(c, v), key);
+        idx' := idx;
+      }
+//      assert v'.maps[idx'][key] == v.maps[idx][key];  // hey look same values
+
+      // Tie from particular map up to abstraction
+      AnyHostWithKeyIsKeyHolder(c, v', idx', key);
+      AnyHostWithKeyIsKeyHolder(c, v, idx, key);
+    }
+
+    assert KnownKeys(c, v') == Types.AllKeys() by {
+      assert KnownKeys(c, v') == Abstraction(c, v').mapp.Keys;  // trigger
+      assert KnownKeys(c, v) == Abstraction(c, v).mapp.Keys;    // trigger
+    }
+    assert MapSpec.NextStep(Abstraction(c, v), Abstraction(c, v'), MapSpec.NoOpStep); // witness
+//#end-elide
+  }
+
+  // This is your proof goal.
+  // You'll need a case analysis on the different kinds of steps to prove
+  // it.
+  lemma RefinementNext(c: Constants, v: Variables, v': Variables)
+    requires Inv(c, v)
+    requires Next(c, v, v')
+    ensures Inv(c, v')
+    ensures MapSpec.Next(Abstraction(c, v), Abstraction(c, v'))
+  {
+    // Use InsertPreservesInvAndRefines, QueryPreservesInvAndRefines, and
+    // TransferPreservesInvAndRefines here to complete this proof.
+//#start-elide
+    var step :| NextStep(c, v, v', step);
+    match step
+      case AcceptRequestStep(request) => {
+        EqualMapsEqualKeysHeldUniquely(c, v, v');
+        EqualMapsEqualMapp(c, v, v');
+        assert MapSpec.NextStep(Abstraction(c, v), Abstraction(c, v'), MapSpec.AcceptRequestStep(request)); // witness
+      }
+      case DeliverReplyStep(request) => {
+        EqualMapsEqualKeysHeldUniquely(c, v, v');
+        EqualMapsEqualMapp(c, v, v');
+        assert MapSpec.NextStep(Abstraction(c, v), Abstraction(c, v'), MapSpec.DeliverReplyStep(request)); // witness
+      }
+      case InsertStep(idx, request) => {
+        InsertPreservesInvAndRefines(c, v, v', idx, request);
+      }
+      case QueryStep(idx, request, output) => {
+        QueryPreservesInvAndRefines(c, v, v', idx, request, output);
+      }
+      case TransferStep(sendIdx, recvIdx, key, value) => {
+        TransferPreservesInvAndRefines(c, v, v', sendIdx, recvIdx, key, value);
+      }
+//#end-elide
   }
 }
